\chapter{De Morgan's Laws. (Finite Dimention Vector Spaces Case)}

\prob{
    Let $V$ be a vector space over a field $\F$ of finite dimension. 
    Let $A, B \subset V$ be vector subspaces. Prove that
    
    \begin{align}
            (A \wedge B)^\perp  &=  \paren{A^\perp \vee B^\perp} \label{p:orthogonal_de_morgan_first}\\
            \intertext{\center{and}}
            (A \vee B)^\perp    &=  \paren{A^\perp \wedge B^\perp} \label{p:orthogonal_de_morgan_second}\\ 
    \end{align}
}

\begin{proof}
    We are going to start with \eqref{p:orthogonal_de_morgan_first}.\pn
    
    First, let see that $\paren{A^\perp \vee B^\perp} \subset (A \wedge B)^\perp$.\pn
    
    Let be $a' \in A^\perp$, $b' \in B^\perp$ and $\lambda_1,\lambda_2 \in \F$. So $\paren{\lambda_1 a' + \lambda_2 b'} \in \paren{A^\perp \vee B^\perp}$. 
    And let be $c \in \paren{A \cap B}$. We have that\pn
    
    \begin{align}
            c \cdot (\lambda_1 a' + \lambda_2 b')   &=  \lambda_1 c \cdot a' + \lambda_2 c \cdot b'     \\
                                                    &=  0   +   \lambda_2 c \cdot b'                    \\
                                                    &\comment{because $c \in A$ and $a' \in A^\perp$}   \\
                                                    &=  0   +   0                                       \\
                                                    &\comment{because $c \in B$ and $a' \in B^\perp$}.   \\
    \end{align}\pn
    
    So, $\paren{A^\perp \vee B^\perp} \subset (A \wedge B)^\perp$, as we wanted.\pn
    
		Now we want to show that $(A \wedge B)^\perp \subset \paren{A^\perp \vee B^\perp}$. It is sufficient to 
		prove that $ \paren{A^\perp \vee B^\perp}^\perp \subset (A \wedge B)$. So, let $x \notin \paren{ A\wedge B }$.	 So $x \notin A$ or $x \notin B$. Without loss of generality suppose that $x \notin A$, so there should be
		$a' \in A^\perp$ such that $x \cdot a' \neq 0$. Now, $a' \in A^\perp \subset \paren{A^\perp \vee B^\perp}$,
		which means that there is an element in $\paren{A^\perp \vee B^\perp}$ that is not orthogonal to $x$. So
		$x \notin \paren{A^\perp \vee B^\perp}^\perp$.\pn
		
    
    For \eqref{p:orthogonal_de_morgan_second} we are going to use the fact that if $C \subset V$ is a vector subspace then
    $(C^\perp)^\perp = C$ (this holds whenever $V$ is a closed vector space, in particular, when $V$ is finite dimensional).
    
    \begin{align}
        (A^\perp \wedge B^\perp)^\perp  &=  (A^\perp)^\perp \vee (B^\perp)^\perp                            \\
                                        &\comment{Here we used \eqref{p:orthogonal_de_morgan_first}}        \\
                                        &=  A \vee B                                                        \\
                                        &\comment{Because of the previously mentioned fact}.
    \end{align}\pn
    
    Using the mentioned fact again, we obtain
    \begin{align}
        A^\perp \wedge B^\perp      &=  \paren{\paren{A^\perp \wedge B^\perp}^\perp}^\perp    \\
                                    &=  \paren{A \vee B}.
    \end{align}\pn
    
    As we wished to prove.
\end{proof}